src/cbor/pulse/raw/everparse/CBOR.Pulse.Raw.EverParse.Iterator.C.fst
@@ -1,0 +1,134 @@
+module CBOR.Pulse.Raw.EverParse.Iterator.C
+#lang-pulse
+open CBOR.Spec.Util
+open CBOR.Pulse.Raw.Util
+open CBOR.Pulse.Raw.Iterator.C
+open Pulse.Lib.Slice open Pulse.Lib.Pervasives open Pulse.Lib.Trade
+
+module PM = Pulse.Lib.SeqMatch
+module A = Pulse.Lib.ArrayPtr
+module S = Pulse.Lib.Slice
+module R = Pulse.Lib.Reference
+module SZ = FStar.SizeT
+module Trade = Pulse.Lib.Trade.Util
+module LP = LowParse.Pulse.VCList
+module LPC = LowParse.Pulse.C
+module U64 = FStar.UInt64
+module SliceIter = CBOR.Pulse.Raw.EverParse.Iterator
+
+let cbor_raw_serialized_iterator_match
+  (#elt_high: Type0)
+  (#k: LP.parser_kind)
+  (#p: LP.parser k elt_high)
+  (s: LP.serializer p { k.parser_kind_subkind == Some LP.ParserStrong })
+  (pm: perm)
+  (c: cbor_raw_serialized_iterator)
+  (l: list elt_high)
+: Tot slprop
+= exists* l' . LPC.pts_to_serialized (LP.serialize_nlist c.glen s) c.s #(pm *. c.p) l' ** pure (
+     SZ.v c.slen == Seq.length (LP.serialize (LP.serialize_nlist c.glen s) l') /\
+     U64.v c.len <= c.glen /\
+     l == fst (List.Tot.splitAt (U64.v c.len) l')
+  )
+
+inline_for_extraction
+fn cbor_raw_serialized_iterator_match_unfold
+  (#elt_high: Type0)
+  (#k: Ghost.erased LP.parser_kind)
+  (#p: LP.parser k elt_high)
+  (s: LP.serializer p)
+  (sq: squash ((Ghost.reveal k).parser_kind_subkind == Some LP.ParserStrong))
+  (pm: perm)
+  (c: cbor_raw_serialized_iterator)
+  (l: Ghost.erased (list elt_high))
+requires
+  cbor_raw_serialized_iterator_match s pm c l
+returns res: SliceIter.cbor_raw_serialized_iterator
+ensures
+  SliceIter.cbor_raw_serialized_iterator_match s pm res l **
+  Trade.trade
+    (SliceIter.cbor_raw_serialized_iterator_match s pm res l)
+    (cbor_raw_serialized_iterator_match s pm c l)
+{
+  unfold (cbor_raw_serialized_iterator_match s pm c l);
+  with l' . assert (LPC.pts_to_serialized (LP.serialize_nlist c.glen s) c.s #(pm *. c.p) l');
+  intro
+    (Trade.trade
+      (LPC.pts_to_serialized (LP.serialize_nlist c.glen s) c.s #(pm *. c.p) l')
+      (cbor_raw_serialized_iterator_match s pm c l)
+    )
+    fn _ {
+      fold (cbor_raw_serialized_iterator_match s pm c l)
+    };
+  let cs = LPC.pts_to_serialized_arrayptr_to_slice
+    #(LP.parse_nlist_kind c.glen k) #(LP.nlist c.glen elt_high) #(coerce_eq () (LP.parse_nlist c.glen p))
+    (coerce_eq () (LP.serialize_nlist c.glen s <: LP.serializer (LP.parse_nlist c.glen p)))
+    c.s c.slen;
+  Trade.trans _ _ (cbor_raw_serialized_iterator_match s pm c l);
+  let res : SliceIter.cbor_raw_serialized_iterator = {
+    s = cs;
+    p = c.p /. 2.0R;
+    glen = c.glen;
+    len = c.len;
+  };
+  SliceIter.cbor_raw_serialized_iterator_fold_with_perm s c.glen _ _ l' res pm l;
+  Trade.trans _ _ (cbor_raw_serialized_iterator_match s pm c l);
+  res
+}
+
+inline_for_extraction
+fn cbor_raw_serialized_iterator_match_fold
+  (#elt_high: Type0)
+  (#k: Ghost.erased LP.parser_kind)
+  (#p: LP.parser k elt_high)
+  (s: LP.serializer p)
+  (sq: squash ((Ghost.reveal k).parser_kind_subkind == Some LP.ParserStrong))
+  (pm: perm)
+  (c: SliceIter.cbor_raw_serialized_iterator)
+  (l: Ghost.erased (list elt_high))
+requires
+  SliceIter.cbor_raw_serialized_iterator_match s pm c l
+returns res: cbor_raw_serialized_iterator
+ensures
+  cbor_raw_serialized_iterator_match s pm res l **
+  Trade.trade
+    (cbor_raw_serialized_iterator_match s pm res l)
+    (SliceIter.cbor_raw_serialized_iterator_match s pm c l)
+{
+  SliceIter.cbor_raw_serialized_iterator_unfold s pm c l;
+  with l' . assert (LP.pts_to_serialized (LP.serialize_nlist (c.glen) s) c.s #(pm *. c.p) l');
+  LP.pts_to_serialized_length (LP.serialize_nlist (c.glen) s) c.s;
+  let a = LPC.pts_to_serialized_slice_to_arrayptr #(LP.parse_nlist_kind c.glen k) #(LP.nlist c.glen elt_high) #(coerce_eq () (LP.parse_nlist c.glen p))
+    (coerce_eq () (LP.serialize_nlist c.glen s <: LP.serializer (LP.parse_nlist c.glen p)))
+    c.s;
+  Trade.trans _ _ (SliceIter.cbor_raw_serialized_iterator_match s pm c l);
+  LPC.pts_to_serialized_share
+    (LP.serialize_nlist (c.glen) s) a;
+  let res : cbor_raw_serialized_iterator = {
+    s = a;
+    slen = S.len c.s;
+    p = c.p /. 2.0R;
+    glen = c.glen;
+    len = c.len;
+  };
+  rewrite
+    (LPC.pts_to_serialized (LP.serialize_nlist c.glen s) a #((pm *. c.p) /. 2.0R) l')
+    as (LPC.pts_to_serialized (LP.serialize_nlist c.glen s) res.s #(pm *. res.p) l');
+  fold (cbor_raw_serialized_iterator_match s pm res l);
+  intro
+    (Trade.trade
+      (cbor_raw_serialized_iterator_match s pm res l)
+      (LPC.pts_to_serialized (LP.serialize_nlist (c.glen) s) a #(pm *. c.p) l')
+    )
+    #(LPC.pts_to_serialized (LP.serialize_nlist c.glen s) a #((pm *. c.p) /. 2.0R) l')
+    fn _ {
+      unfold (cbor_raw_serialized_iterator_match s pm res l);
+      with pm2 l2 . rewrite (LPC.pts_to_serialized (LP.serialize_nlist (c.glen) s) res.s #pm2 l2)
+        as (LPC.pts_to_serialized (LP.serialize_nlist (c.glen) s) a #pm2 l2);
+      LPC.pts_to_serialized_gather
+        (LP.serialize_nlist (c.glen) s) a;
+      ()
+    };
+  Trade.trans _ _ (SliceIter.cbor_raw_serialized_iterator_match s pm c l);
+  res
+}
